\documentclass{scrartcl}
\usepackage{amsmath}
\usepackage{amssymb}
\usepackage[geometry]{ifsym}
\usepackage{graphicx}
\usepackage[outputdir=build]{minted}

\newcommand{\selection}{\sigma}
\newcommand{\projection}{\pi}
\newcommand{\rename}{\rho}
\newcommand{\join}{\mathbin{\text{\begin{tiny}\textifsym{|><|}\end{tiny}}}}
\newcommand{\fullouterjoin}{\mathbin{\text{\begin{tiny}\textifsym{d|><|d}\end{tiny}}}}
\newcommand{\leftouterjoin}{\mathbin{\text{\begin{tiny}\textifsym{d|><|}\end{tiny}}}}
\newcommand{\rightouterjoin}{\mathbin{\text{\begin{tiny}\textifsym{|><|d}\end{tiny}}}}
\newcommand{\semijoin}{\mathbin{\text{\begin{tiny}\textifsym{|><}\end{tiny}}}}
\newcommand{\groupby}{\Gamma}

\newcommand{\mtt}[1]{\text{\texttt{#1}}}

\setlength{\parindent}{0pt}

\begin{document}

\section*{Exercise 1}
\subsection*{a}
\begin{align*}
  {n \choose k} = \frac{n!}{k!(n-k)!} = \frac{n!}{(n-k)!(n - (n-k))!} = {n \choose n-k}
\end{align*}

\subsection*{b}
\begin{align*}
  {n - 1 \choose k} + {n - 1 \choose k - 1}  = \frac{(n-1)!}{k!((n-1)-k)!} + \frac{(n - 1)!}{(k-1)!((n - 1) - (k-1))!} = \\
  = (n-1)!\left( \frac{n-k}{k!(n-k)!} + \frac{k}{k!(n-k)!} \right) = (n-1)!\left( \frac{n}{k!(n-k)!} \right) = \\
  \frac{n(n-1)!}{k!(n-k)!} = \frac{n!}{k!(n-k)!} = {n \choose k}
\end{align*}


\end{document}
